Skeleton for single disk on top of two disks
Without crashes this implementation is of course silly, but already
illustrates that we will need invariants over implementations: the
abstraction function and simulation more generally can't handle an
arbitrary state, but need to rely on some invariants (in this case, to
write to both disks requires that they have the same domain).

Refinement/TwoDiskAPI.v
@@ -1,5 +1,4 @@
 Require Export Disk.
-Require Import Mem.
 Require Import Implements.
 
 Inductive diskId := d0 | d1.
@@ -25,14 +24,14 @@ Module TDSpec.
     end.
 
   Definition Read i a : Semantics block :=
-    StepRel (fun state v state' =>
-                match get_disk i state a with
-                | Some v0 => v = v0
-                | None => True
-                end /\ state' = state).
+    StepRel (fun state r state' =>
+               match get_disk i state a with
+               | Some v0 => r = v0
+               | None => True
+               end /\ state' = state).
 
   Definition Write i a b : Semantics unit :=
-    StepRel (fun state v state' =>
+    StepRel (fun state r state' =>
                match get_disk i state a with
                | Some v0 => state' = upd_disk i (fun d => upd d a b) state
                | None => True (* new disk is arbitrary *)
