Refinement/SeqDiskAPI.v
@@ -1,0 +1,27 @@
+Require Export Disk.
+Require Import Implements.
+
+Module DSpec.
+  Record State :=
+    Disk { sdisk : disk }.
+
+  Definition Read a : Semantics block :=
+    StepRel (fun state r state' =>
+               match sdisk state a with
+               | Some v0 => r = v0
+               | None => True
+               end /\ state' = state).
+
+  Definition Write a b : Semantics unit :=
+    StepRel (fun state r state' =>
+               match sdisk state a with
+               | Some v0 => state' = Disk (upd (sdisk state) a b) /\
+                           r = tt
+               | None => True
+               end).
+
+End DSpec.
+
+(* Local Variables: *)
+(* company-coq-local-symbols: (("State" . ?Σ) ("state" . ?σ) ("state'" . (?σ (Br . Bl) ?'))) *)
+(* End: *)
