Refinement/SeqDiskImpl.v
@@ -1,0 +1,54 @@
+Require Import Refinement.IO.
+Require Import TwoDiskAPI TwoDiskImpl.
+Require Import SeqDiskAPI.
+Require Import Implements.
+Require Import Automation.
+
+(* D is an implementation of the single, sequential disk in DSpec. *)
+Module D.
+  Definition Read a :=
+    v0 <- TD.Read d0 a;
+      Ret v0.
+  Definition Write a b :=
+    _ <- TD.Write d0 a b;
+      _ <- TD.Write d1 a b;
+      Ret tt.
+
+  Definition abstraction : TDSpec.State -> DSpec.State :=
+    fun ds => DSpec.Disk (TDSpec.disk0 ds).
+
+  Theorem Read_ok : forall a,
+      implements
+        (DSpec.Read a)
+        (io_semantics (Read a))
+        (fun w => abstraction (TD.abstraction w)).
+  Proof.
+    intros.
+    unfold implements; simpl; intros.
+    unfold Read in H.
+    step.
+    step.
+    eapply TD.Read_ok in H; simpl in H; safe_intuition.
+    destruct matches; intuition subst; try congruence.
+  Qed.
+
+  Theorem Write_ok : forall a b,
+      implements
+        (DSpec.Write a b)
+        (io_semantics (Write a b))
+        (fun w => abstraction (TD.abstraction w)).
+  Proof.
+    intros.
+    unfold implements; simpl; intros.
+    unfold Write in H.
+    repeat step.
+    repeat match goal with
+           | [ H: io_step (TD.Write _ _ _) _ _ _ |- _ ] =>
+             eapply TD.Write_ok in H; simpl in H; safe_intuition
+           end.
+    destruct matches; intuition subst.
+    (* actually need to know invariant that domains are equal; implements
+     relation should incorporate an invariant over the impl states *)
+  Abort.
+
+End D.
